add powerful sig elim rule and ceq; prove pair_eta

MiniPRL.v
@@ -4,9 +4,11 @@
    [1]: https://github.com/jozefg/miniprl
    [2]: http://www.nuprl.org/html/Nuprl2Coq/ *)
 Require String.
-Require Import List Arith Bool Omega.
+Require Import List Bool Arith.
+Require Omega. (* do not import; conflicts with "~" notation *)
 Import ListNotations.
 
+Ltac omega := Omega.omega. (* sigh... *)
 
 From StructTact Require Import StructTactics Assoc BoolUtil.
 
@@ -35,6 +37,9 @@ Module expr.
   | Unit : t
 
   | Eq : t -> t -> t -> t
+
+  | Ceq : t -> t -> t
+
   | Uni (level : nat) : t
 
   | Cust : guid.t -> t
@@ -64,6 +69,8 @@ Module expr.
     Notation "A * B" := (expr.Sig A B) : expr_scope.
     Notation "A = B 'in' C" := (expr.Eq A B C) (at level 70, B at next level) : expr_scope.
 
+    Notation "A ~ B" := (expr.Ceq A B) (at level 70) : expr_scope.
+
     Local Open Scope expr.
     Import exports.
 
@@ -73,6 +80,8 @@ Module expr.
     Check (0, 0).
     Check (\ 0) * (\ 0).
     Check (\ 0) = (\ 0) in Unit.
+    Check ((\ 0) ~ (\ 0) )%expr.
+
   End notations.
 
   (* The rest of this module defines some fundamental operations on the syntax,
@@ -90,6 +99,7 @@ Module expr.
     | tt => tt
     | Unit => Unit
     | Eq e1 e2 e3 => Eq (lift c d e1) (lift c d e2) (lift c d e3)
+    | Ceq e1 e2 => Ceq (lift c d e1) (lift c d e2)
     | Uni i => Uni i
     | Cust g => Cust g
     end.
@@ -112,6 +122,7 @@ Module expr.
     | tt => tt
     | Unit => Unit
     | Eq e1 e2 e3 => Eq (subst e1 from to) (subst e2 from to) (subst e3 from to)
+    | Ceq e1 e2 => Ceq (subst e1 from to) (subst e2 from to)
     | Uni i => Uni i
     | Cust g => Cust g
     end.
@@ -135,6 +146,7 @@ Module expr.
       | tt => True
       | Unit => True
       | Eq e1 e2 e3 => t n e1 /\ t n e2 /\ t n e3
+      | Ceq e1 e2 => t n e1 /\ t n e2
       | Uni i => True
       | Cust g => True
       end.
@@ -190,6 +202,14 @@ Module expr.
                    end
         | right _ => right _
         end
+      | Ceq e1 e2 =>
+        match dec n e1 with
+        | left _ => match dec n e2 with
+                   | left _ => left (conj _ _)
+                   | right _ => right _
+                   end
+        | right _ => right _
+        end
       | Uni i => left I
       | Cust g => left I
       end; simpl; intuition.
@@ -233,7 +253,7 @@ Module expr.
     Qed.
 
     Lemma lift':
-      forall (n d : nat) (a : expr.t), t n a -> t (d + n) (expr.lift 0 d a).
+      forall (n c d : nat) (a : expr.t), t n a -> t (d + n) (expr.lift c d a).
     Proof.
       intros. rewrite <- Nat.add_comm. apply lift.  auto.
     Qed.
@@ -257,23 +277,257 @@ Module expr.
   End wf.
 End expr.
 
-Module telescope.
-  Definition t := list expr.t.
+Module value.
+  Inductive t : expr.t -> Prop :=
+  | Lam : forall e, t (expr.Lam e)
+  | Pi : forall e1 e2, t (expr.Pi e1 e2)
+  | tt : t expr.tt
+  | Unit : t expr.Unit
+  | Eq : forall e1 e2 e3, t (expr.Eq e1 e2 e3)
+  | Ceq : forall e1 e2, t (expr.Ceq e1 e2)
+  | Uni : forall i, t (expr.Uni i)
+  | Cust : forall g, t (expr.Cust g)
+  | Pair : forall e1 e2, t (expr.Pair e1 e2)
+  | Sig : forall e1 e2, t (expr.Sig e1 e2)
+  .
+  Hint Constructors t.
+End value.
 
-  Definition empty : t := [ ].
+Module step.
+  Module result.
+    Inductive t :=
+    | Step : expr.t -> t
+    | Value : t
+    | Stuck : t
+    .
+  End result.
+
+  Inductive t : expr.t -> expr.t -> Prop :=
+  | Beta : forall e1 e2, t (expr.App (expr.Lam e1) e2) (expr.subst e1 0 e2)
+  | AppL : forall e1 e1' e2, t e1 e1' -> t (expr.App e1 e2) (expr.App e1' e2)
+  | FstPair : forall e1 e2, t (expr.Fst (expr.Pair e1 e2)) e1
+  | SndPair : forall e1 e2, t (expr.Snd (expr.Pair e1 e2)) e2
+  | Fst : forall e e', t e e' -> t (expr.Fst e) (expr.Fst e')
+  | Snd : forall e e', t e e' -> t (expr.Snd e) (expr.Snd e')
+  .
+  Hint Constructors t.
+
+  Lemma det : forall e e1 e2, t e e1 -> t e e2 -> e1 = e2.
+  Proof.
+    intros.
+    generalize dependent e2.
+    induction H; intros.
+    - invc H0.
+      + auto.
+      + solve_by_inversion.
+    - invc H0.
+      + solve_by_inversion.
+      + f_equal; auto.
+    - invc H0.
+      + auto.
+      + solve_by_inversion.
+    - invc H0.
+      + auto.
+      + solve_by_inversion.
+    - invc H0.
+      + solve_by_inversion.
+      + f_equal; auto.
+    - invc H0.
+      + solve_by_inversion.
+      + f_equal; auto.
+  Qed.
+
+  Fixpoint f (e : expr.t) : result.t :=
+    match e with
+    | expr.Var n => result.Stuck
+    | expr.Lam e => result.Value
+    | expr.App e1 e2 =>
+      match f e1 with
+      | result.Stuck => result.Stuck
+      | result.Value => match e1 with
+                       | expr.Lam e1 => result.Step (expr.subst e1 0 e2)
+                       | _ => result.Stuck
+                       end
+      | result.Step e1' => result.Step (expr.App e1' e2)
+      end
+    | expr.Pi e1 e2 => result.Value
+    | expr.Pair e1 e2 => result.Value
+    | expr.Fst e =>
+      match f e with
+      | result.Stuck => result.Stuck
+      | result.Value => match e with
+                       | expr.Pair e1 e2 => result.Step e1
+                       | _ => result.Stuck
+                       end
+      | result.Step e' => result.Step (expr.Fst e')
+      end
+    | expr.Snd e =>
+      match f e with
+      | result.Stuck => result.Stuck
+      | result.Value => match e with
+                       | expr.Pair e1 e2 => result.Step e2
+                       | _ => result.Stuck
+                       end
+      | result.Step e' => result.Step (expr.Snd e')
+      end
+    | expr.Sig e1 e2 => result.Value
+    | expr.tt => result.Value
+    | expr.Unit => result.Value
+    | expr.Eq e1 e2 e3 => result.Value
+    | expr.Ceq e1 e2 => result.Value
+    | expr.Uni i => result.Value
+    | expr.Cust g => result.Value
+    end.
+
+  Lemma f_t :
+    forall e, match f e with
+         | result.Step e' => t e e'
+         | result.Value => value.t e
+         | result.Stuck => (forall e', ~ t e e') /\ ~ value.t e
+         end.
+  Proof.
+    induction e; simpl; auto.
+    - intuition; solve_by_inversion.
+    - destruct (f e1).
+      + auto.
+      + invcs IHe1; intuition; invc H; try solve_by_inversion.
+      + intuition; invc H1; eauto.
+    - destruct (f e).
+      + auto.
+      + invcs IHe; intuition; invc H; try solve_by_inversion.
+      + intuition; invc H1; eauto.
+    - destruct (f e).
+      + auto.
+      + invcs IHe; intuition; invc H; try solve_by_inversion.
+      + intuition; invc H1; eauto.
+  Qed.
+End step.
+
+Module star.
+  Definition t : expr.t -> expr.t -> Prop := Relation_Operators.clos_refl_trans_1n _ step.t.
+End star.
+
+Module eval.
+  Definition t (e : expr.t) (v : expr.t) : Prop :=
+    star.t e v /\ value.t v.
+End eval.
+
+Module run.
+  Fixpoint f (n : nat) (e : expr.t) : option expr.t :=
+    match n with
+    | 0 => Some e
+    | S n => match step.f e with
+            | step.result.Step e' => f n e'
+            | step.result.Value => Some e
+            | step.result.Stuck => None
+            end
+    end.
+End run.
+
+Lemma nth_error_firstn_skipn:
+  forall (A : Type) (C : list A) (i : nat) (e : A),
+    nth_error C i = Some e -> firstn i C ++ e :: skipn (S i) C = C.
+Proof.
+  induction C; destruct i; intros; try discriminate.
+  - simpl in *. congruence.
+  - simpl in H. apply IHC in H.
+    change (firstn _ _) with (a :: firstn i C).
+    change (skipn _ _) with (skipn (S i) C).
+    cbn [app].
+    now rewrite H.
+Qed.
+
+Lemma firstn_skipn_length :
+  forall A n (l : list A), length (firstn n l) + length (skipn n l) = length l.
+Proof.
+  intros.
+  rewrite <- app_length.
+  f_equal.
+  apply firstn_skipn.
+Qed.
+
+
+Lemma firstn_snoc :
+  forall A n l (a : A),
+    nth_error l n = Some a ->
+    firstn n l ++ [a] = firstn (S n) l.
+Proof.
+  induction n; destruct l; intros.
+  - simpl in *. discriminate.
+  - simpl in *. congruence.
+  - simpl in *. discriminate.
+  - simpl in H. apply IHn in H.
+    change (firstn (S n) _) with (a :: firstn n l).
+    change (firstn (S (S n)) _) with (a :: firstn (S n) l).
+    cbn [app].
+    auto using f_equal.
+Qed.
+
+Module binding.
+  Definition t (E : Type) : Type := String.string * E.
+End binding.
+
+Module outermost_first_telescope.
+  (* The head of the list is the *least* recently bound variable. *)
+  Definition t E := list (binding.t E).
+
+  Fixpoint lift (c d : nat) (C : t expr.t) : t expr.t :=
+    match C with
+    | [] => []
+    | (n,e) :: C => (n, expr.lift c d e) :: lift (S c) d C
+    end.
+
+  Fixpoint subst (C : t expr.t) (from : nat) (to : expr.t) : t expr.t :=
+    match C with
+    | [] => []
+    | (n, e) :: C => (n, expr.subst e from to) :: subst C (S from) (expr.lift 0 1 to)
+    end.
+
+  Module wf.
+    Fixpoint t (k : nat) (C : t expr.t) : Prop :=
+      match C with
+      | [] => True
+      | (_, e) :: C => expr.wf.t k e /\ t (S k) C
+      end.
+
+    Lemma app : forall C1 C2 n,
+        outermost_first_telescope.wf.t n C1 ->
+        outermost_first_telescope.wf.t (n + length C1) C2 ->
+        outermost_first_telescope.wf.t n (C1 ++ C2).
+    Proof.
+      induction C1; simpl; repeat break_match; intuition.
+      - eapply eq_rect with (P := fun x => _ x _); eauto.
+      - apply IHC1; auto.
+        eapply eq_rect with (P := fun x => _ x _); eauto.
+        omega.
+    Qed.
+  End wf.
+End outermost_first_telescope.
+
+Module telescope.
+  (* The head of the list is the *most* recently bound variable. *)
+  Definition t E := list (binding.t E).
+
+  Definition names E (C : t E) : list String.string := map (@fst _ _) C.
 
   (* Looking up an element of the telescope lifts the answer so that it is well
      formed in the telescope of *all* bindings of the telescope. *)
-  Fixpoint nth (C : t) (i : nat) : option expr.t :=
+  Fixpoint nth (C : t expr.t) (i : nat) : option expr.t :=
     match C with
-    | nil => None
-    | cons e C => match i with
+    | [] => None
+    | (n, e) :: C => match i with
                  | 0 => Some (expr.lift 0 1 e)
                  | S i => match nth C i with
                          | None => None
                          | Some e => Some (expr.lift 0 1 e)
                          end
                  end
+    end.
+
+  Definition split E (C : t E) (i : nat) : option (t E * binding.t E * t E) :=
+    match nth_error C i with
+    | None => None
+    | Some e => Some (firstn i C, e, skipn (S i) C)
     end.
 
   Lemma nth_length C : forall i e, nth C i = Some e -> i < length C.
@@ -285,36 +539,151 @@ Module telescope.
       + find_inversion. eauto using lt_n_S.
   Qed.
 
+  Lemma split_app : forall E C i C1 (e : binding.t E) C2,
+      split C i = Some (C1, e, C2) ->
+      C1 ++ e :: C2 = C.
+  Proof.
+    unfold split.
+    intros.
+    break_match; try discriminate.
+    match goal with
+    | [ H : Some (?a, ?b, ?c) = Some (?d, ?e, ?f) |- _ ] =>
+      (assert (a = d /\ b = e /\ c = f) by (intuition congruence)); clear H; repeat break_and; subst
+    end.
+    auto using nth_error_firstn_skipn.
+  Qed.
+
+  Definition to_outer E (C : t E) : outermost_first_telescope.t E := rev C.
+  Definition from_outer E (C : outermost_first_telescope.t E) : t E := rev C.
+
+  Definition lift (c d : nat) (C : t expr.t) : t expr.t :=
+    from_outer (outermost_first_telescope.lift c d (to_outer C)).
+
+  Definition subst (C : t expr.t) (from : nat) (to : expr.t) : t expr.t :=
+    from_outer (outermost_first_telescope.subst (to_outer C) from to).
+
   Module wf.
-    Fixpoint t (k : nat) (C : telescope.t) : Prop :=
+    Fixpoint t (k : nat) (C : t expr.t) : Prop :=
       match C with
       | [] => True
-      | e :: C => t k C /\ expr.wf.t (k + length C) e
+      | (_,e) :: C => t k C /\ expr.wf.t (k + length C) e
       end.
-  End wf.
 
-  Lemma nth_wf :
-    forall C k i e,
-      wf.t k C ->
-      nth C i = Some e ->
-      expr.wf.t (k + length C) e.
-  Proof.
-    induction C; intros; destruct i; simpl in *; try discriminate.
-    - find_inversion. break_and.
-      rewrite <- plus_n_Sm.
-      auto using expr.wf.lift_0_1.
-    - break_and. break_match; try discriminate.
-      find_inversion.
-      rewrite <- plus_n_Sm.
-      eauto using expr.wf.lift_0_1.
-  Qed.
+    Lemma nth :
+      forall C k i e,
+        nth C i = Some e ->
+        wf.t k C ->
+        expr.wf.t (k + length C) e.
+    Proof.
+      induction C; intros; destruct i; simpl in *; repeat break_let; try discriminate.
+      - find_inversion. break_and.
+        rewrite <- plus_n_Sm.
+        auto using expr.wf.lift_0_1.
+      - break_and. break_match; try discriminate.
+        find_inversion.
+        rewrite <- plus_n_Sm.
+        eauto using expr.wf.lift_0_1.
+    Qed.
+
+    Lemma firstn :
+      forall (n : nat) C (k : nat), wf.t k C -> wf.t (length (skipn n C) + k) (firstn n C).
+    Proof.
+      induction n; simpl; intros.
+      + auto.
+      + break_match; simpl in *; repeat break_let; intuition.
+        pose proof firstn_skipn_length n t1.
+        eapply eq_rect with (P := fun x => expr.wf.t x _).
+        eauto.
+        omega.
+    Qed.
+
+    Lemma skipn :
+      forall (n : nat) C (k : nat), wf.t k C -> wf.t k (skipn n C).
+    Proof.
+      induction n; simpl; intros.
+      + auto.
+      + break_match; simpl in *; repeat break_let; intuition.
+    Qed.
+
+
+    Lemma app_inv :
+      forall C1 C2 k,
+        wf.t k (C1 ++ C2) ->
+        wf.t (length C2 + k) C1 /\ wf.t k C2.
+    Proof.
+      induction C1; simpl; intros.
+      - intuition.
+      - repeat break_let. break_and.
+        apply IHC1 in H. break_and.
+        intuition.
+        rewrite app_length in *.
+        eapply eq_rect with (P := fun x => _ x _); eauto.
+        omega.
+    Qed.
+
+    Lemma split : forall C k i C1 n e C2,
+        split C i = Some (C1, (n, e), C2) ->
+        wf.t k C ->
+        wf.t (S (length C2 + k)) C1 /\ expr.wf.t (length C2 + k) e /\ wf.t k C2.
+    Proof.
+      unfold split.
+      intros.
+      break_match; try discriminate.
+      match goal with
+      | [ H : Some (?a, ?b, ?c) = Some (?d, ?e, ?f) |- _ ] =>
+        (assert (a = d /\ b = e /\ c = f) by (intuition congruence));
+        clear H; repeat break_and; subst
+      end.
+      pose proof nth_error_firstn_skipn _ _ Heqo.
+      rewrite <- H in H0.
+      apply app_inv in H0. break_and.
+      cbn [wf.t] in H1. break_and.
+      cbn [length] in *.
+      intuition.
+      eapply eq_rect with (P := fun x => _ x _); eauto.
+      omega.
+    Qed.
+
+    Lemma app :
+      forall C1 C2 k,
+        wf.t (length C2 + k) C1 ->
+        wf.t k C2 ->
+        wf.t k (C1 ++ C2).
+    Proof.
+      induction C1; simpl; repeat break_let; intuition.
+      rewrite app_length.
+      eapply eq_rect with (P := fun x => _ x _); eauto.
+      omega.
+    Qed.
+
+    Lemma to_outer_wf : forall C n, telescope.wf.t n C -> outermost_first_telescope.wf.t n (to_outer C).
+    Proof.
+      unfold to_outer.
+      induction C; intros.
+      - auto.
+      - simpl in H. break_let; break_and. simpl.
+        apply outermost_first_telescope.wf.app; auto.
+        simpl. rewrite rev_length. auto.
+    Qed.
+
+    Lemma from_outer_wf : forall C n, outermost_first_telescope.wf.t n C -> telescope.wf.t n (from_outer C).
+    Proof.
+      unfold from_outer.
+      induction C; intros.
+      - auto.
+      - simpl in H. break_let; break_and. simpl.
+        apply telescope.wf.app; simpl.
+        apply IHC. auto.
+        rewrite <- plus_n_O. auto.
+    Qed.
+  End wf.
 End telescope.
 
 Module sequent.
-  Record t : Type :=
+  Record t E : Type :=
     Make {
-        context : telescope.t;
-        goal : expr.t
+        context : telescope.t E;
+        goal : E
     }.
 
   Module notations.
@@ -326,7 +695,7 @@ Module sequent.
   Module wf.
     Import notations.
     Local Open Scope sequent.
-    Definition t (S : sequent.t) : Prop :=
+    Definition t (S : sequent.t expr.t) : Prop :=
       match S with
       | H >> C => telescope.wf.t 0 H /\ expr.wf.t (length H) C
       end.
@@ -358,6 +727,13 @@ Module derivation.
   | Eq_Mem_Eq : t -> t
   | Eq_Sym : t -> t
   | Eq_Subst (i : nat) (a : expr.t) (D_ty : t) (D_eq D_body : t) : t
+
+  | Ceq_Eq (D_lhs D_rhs : t) : t
+  | Ceq_Mem_Eq (D : t) : t
+  | Ceq_Sym (D : t) : t
+  | Ceq_Subst (e : expr.t) (D_ceq D_C : t) : t
+  | Ceq_Step (D : t) : t
+  | Ceq_Refl : t
 
   | Uni_Eq : t
   | Cumulative : t -> t
@@ -405,6 +781,12 @@ Module derivation.
       | derivation.Eq_Mem_Eq D => t n D
       | derivation.Eq_Sym D => t n D
       | derivation.Eq_Subst i a D_ty D_eq D_body => False (* TODO *)
+      | derivation.Ceq_Eq D_lhs D_rhs => t n D_lhs /\ t n D_rhs
+      | derivation.Ceq_Mem_Eq D => t n D
+      | derivation.Ceq_Sym D => t n D
+      | derivation.Ceq_Subst e D_ceq D_C => expr.wf.t (S n) e /\ t n D_ceq /\ t n D_C
+      | derivation.Ceq_Step D => t n D
+      | derivation.Ceq_Refl => True
       | derivation.Uni_Eq => True
       | derivation.Cumulative D => t n D
       | derivation.Witness w D => expr.wf.t n w /\ t n D
@@ -438,7 +820,13 @@ Module extract.
     | derivation.Eq_Eq D_ty D_lhs D_rhs => expr.tt
     | derivation.Eq_Mem_Eq D => expr.tt
     | derivation.Eq_Sym D => expr.tt
-    | derivation.Eq_Subst i a D_ty D_eq D_body => f D_body
+    | derivation.Eq_Subst i a D_ty D_eq D_body => expr.tt
+    | derivation.Ceq_Eq D_lhs D_rhs => expr.tt
+    | derivation.Ceq_Mem_Eq D => expr.tt
+    | derivation.Ceq_Sym D => expr.tt
+    | derivation.Ceq_Subst e D_ceq D_C => f D_C
+    | derivation.Ceq_Step D => expr.tt
+    | derivation.Ceq_Refl => expr.tt
     | derivation.Uni_Eq => expr.tt
     | derivation.Cumulative D => expr.tt
     | derivation.Witness w D => w
@@ -552,7 +940,7 @@ End TACTIC.
 
 Module tactic <: TACTIC.
   Definition derivation := derivation.t.
-  Definition goal := sequent.t.
+  Definition goal := sequent.t expr.t.
 
   Definition result := tactic_result.t derivation goal.
 
@@ -563,13 +951,13 @@ Module refiner.
   Module result.
     Inductive t :=
     | Proved : derivation.t -> (* extract: *) expr.t -> t
-    | Incomplete : list sequent.t -> t
+    | Incomplete : list (sequent.t expr.t) -> t
     | Failed : t
     .
   End result.
 
   Definition prove (thm : expr.t) (t : tactic.t) : result.t :=
-    match tactic_monad.run (t _ (sequent.Make telescope.empty thm)) with
+    match tactic_monad.run (t _ (sequent.Make [] thm)) with
     | Some (tactic_result.Make ev gs) =>
       match gs with
       | [] => match ev [] with
@@ -586,6 +974,18 @@ Definition option_bind {A B} (m : option A) (f : A -> option B) : option B :=
   match m with
   | None => None
   | Some a => f a
+  end.
+
+Fixpoint sequence_option {A} (l : list (option A)) : option (list A) :=
+  match l with
+  | [] => Some []
+  | x :: xs => match x with
+              | None => None
+              | Some a => match sequence_option xs with
+                         | None => None
+                         | Some l => Some (a :: l)
+                         end
+              end
   end.
 
 Module primitive_tactics (T : TACTIC).
@@ -619,18 +1019,6 @@ Module primitive_tactics (T : TACTIC).
                   | Some ys => Some (f x :: ys)
                   end
       end
-    end.
-
-  Fixpoint sequence_option {A} (l : list (option A)) : option (list A) :=
-    match l with
-    | [] => Some []
-    | x :: xs => match x with
-                | None => None
-                | Some a => match sequence_option xs with
-                           | None => None
-                           | Some l => Some (a :: l)
-                           end
-                end
     end.
 
   Definition join_evidence (subresults : list T.result) (ds : list T.derivation)
@@ -676,444 +1064,88 @@ End primitive_tactics.
 
 Module P := primitive_tactics tactic.
 
-Module rules.
-  Import P.
-  Import tactic_monad.
-  Local Open Scope tactic_monad.
 
-  Import sequent.notations.
-  Local Open Scope sequent.
+Fixpoint inc_digits (base : nat) (l : list nat) : list nat :=
+  match l with
+  | [] => [1]
+  | d :: l => if base =? (S d) then 0 :: inc_digits base l
+             else S d :: l
+  end.
 
-  Definition nullary_derivation (d : derivation.t) :=
-    tactic_result.Make(G:=sequent.t) (fun _ => Some d) [].
+Fixpoint digits' (base : nat) (acc : list nat) (n : nat) : list nat :=
+  match n with
+  | 0 => acc
+  | S n => digits' base (inc_digits base acc) n
+  end.
 
-  Definition unary_derivation (d : derivation.t -> derivation.t) g :=
-    tactic_result.Make(G:=sequent.t) (fun l => match l with
-                                            | [x]  => Some (d x)
-                                            | _ => None
-                                            end) [g].
+Definition digits (base : nat) (n : nat) : list nat := List.rev (digits' base [0] n).
 
-  Definition binary_derivation (d : derivation.t -> derivation.t -> derivation.t) g1 g2 :=
-    tactic_result.Make(G:=sequent.t)
-      (fun l => match l with
-             | [d1; d2] => Some (d d1 d2)
-             | _ => None
-             end)
-      [g1; g2].
+Definition decimal_digit_to_ascii (d : nat) : Ascii.ascii :=
+  Ascii.ascii_of_nat (48 + d).
 
-  Definition ternary_derivation (d : derivation.t -> derivation.t ->
-                                     derivation.t -> derivation.t) g1 g2 g3 :=
-    tactic_result.Make(G:=sequent.t)
-      (fun l => match l with
-             | [d1; d2; d3] => Some (d d1 d2 d3)
-             | _ => None
-             end)
-      [g1; g2; g3].
+Definition ascii_to_decimal_digit (a : Ascii.ascii) : nat :=
+  Ascii.nat_of_ascii a - 48.
 
-  Module wf.
-    Definition t (rule : tactic.t) : Prop :=
-      forall g res,
-        sequent.wf.t g ->
-        run (rule _ g) = Some res ->
-        tactic_result.wf.t (fun g d => derivation.wf.t (length (sequent.context g)) d) g res /\
-        List.Forall sequent.wf.t (tactic_result.goals res).
-  End wf.
-
-    Ltac head_symbol e :=
-      match e with
-      | ?f ?x => head_symbol f
-      | _ => e
-      end.
-
-    Ltac crush_wf :=
-      match goal with
-      | [ |- wf.t ?f ] => let x := head_symbol f in unfold x
-      end;
-      unfold wf.t;
-      intros;
-      unfold_tactic_monad;
-      repeat break_match; try discriminate;
-      find_inversion;
-      unfold nullary_derivation, unary_derivation, binary_derivation, ternary_derivation;
-      simpl in *; repeat break_and; split; [
-        unfold tactic_result.wf.t; simpl; intros;
-        repeat match goal with
-               | [ H : Forall2 _ _ _ |- _ ] => invc H
-               end;
-        eexists; intuition eauto; simpl in *; intuition;
-        eauto using telescope.nth_length
-      | unfold sequent.wf.t in *;
-        repeat (apply Forall_cons || apply Forall_nil); simpl; intuition;
-        try match goal with
-        | [ H : telescope.nth _ _ = Some _ |- expr.wf.t _ _ ] =>
-          eapply telescope.nth_wf in H; [|solve[eauto]]; simpl in H; intuition
-        end ];
-      auto using expr.wf.subst with arith;
-      try match goal with
-      | [  |- expr.wf.t _ (expr.lift _ ?n _) ] =>
-        solve [apply expr.wf.lift' with (d := n); auto]
-      end.
-
-  Module unit.
-    (* H >> unit = unit in U(i) *)
-    Definition Eq : tactic.t :=
-      fun R g =>
-      match g with
-      | H >> (expr.Eq expr.Unit expr.Unit (expr.Uni _)) =>
-        ret (nullary_derivation derivation.Unit_Eq)
-      | _ => fail
-      end.
-
-    Lemma Eq_wf : wf.t Eq.
-    Proof. crush_wf. Qed.
-
-    (* H >> unit *)
-    Definition Intro : tactic.t :=
-      fun R g =>
-      match g with
-      | H >> expr.Unit => ret (nullary_derivation derivation.Unit_Intro)
-      | _ => fail
-      end.
-
-    Lemma Intro_wf : wf.t Intro.
-    Proof. crush_wf. Qed.
-
-    (* H >> tt = tt in unit *)
-    Definition TTEq : tactic.t :=
-      fun R g =>
-      match g with
-      | H >> (expr.Eq expr.tt expr.tt expr.Unit) =>
-        ret (nullary_derivation derivation.tt_Eq)
-      | _ => fail
-      end.
-
-    Lemma TTEq_wf : wf.t TTEq.
-    Proof. crush_wf. Qed.
-  End unit.
-
-  Module pi.
-
-    (* H >> x:A -> B = x:A' -> B' in U(i)
-         H >> A = A' in U(i)
-         H, x:A >> B = B' in U(i) *)
-    Definition Eq : tactic.t :=
-      fun R g =>
-      match g with
-      | H >> expr.Eq (expr.Pi A B) (expr.Pi A' B') (expr.Uni i) =>
-        ret (binary_derivation derivation.Pi_Eq
-                (H >> (expr.Eq A A' (expr.Uni i)))
-                (A :: H >> (expr.Eq B B' (expr.Uni i))))
-      | _ => fail
-      end.
-
-    Lemma Eq_wf : wf.t Eq.
-    Proof. crush_wf. Qed.
-
-    (* H >> x:A -> B
-         H >> A = A in U(i)
-         H, x:A >> B *)
-    Definition Intro (i : nat) : tactic.t :=
-      fun R g =>
-      match g with
-      | H >> expr.Pi A B =>
-        ret (binary_derivation (derivation.Pi_Intro i)
-                (H >> expr.Eq A A (expr.Uni i))
-                (A :: H >> B))
-      | _ => fail
-      end.
-
-    Lemma Intro_wf i : wf.t (Intro i).
-    Proof. crush_wf. Qed.
-
-    (* H >> C
-         H(n) = x:A -> B
-         H >> e = e in A
-         H, [e/x]B >> C
-     *)
-    Definition Elim (n : nat) (e : expr.t) : tactic.t :=
-      fun R g =>
-      match g with
-      | H >> C =>
-        _ <- assume_sb (expr.wf.dec (length H) e) ;;
-        ty <- unwrap (telescope.nth H n) ;;
-        match ty with
-        | expr.Pi A B =>
-          ret (binary_derivation (derivation.Pi_Elim n e)
-                  (H >> expr.Eq e e A)
-                  (expr.subst B 0 e :: H >> expr.lift 0 1 C))
-        | _ => fail
-        end
-      end.
-
-    Lemma Elim_wf n e : wf.t (Elim n e).
-    Proof. crush_wf. Qed.
-
-    (* H >> \x.e = \x.e' in x:A -> B
-         H >> A = A in U(i)
-         H, x:A >> e = e' in B *)
-    Definition LamEq (i : nat) : tactic.t :=
-      fun R g =>
-      match g with
-      | H >> expr.Eq (expr.Lam e) (expr.Lam e') (expr.Pi A B) =>
-        ret (binary_derivation (derivation.Lam_Eq i)
-                (H >> expr.Eq A A (expr.Uni i))
-                (A :: H >> expr.Eq e e' B))
-      | _ => fail
-      end.
-
-    Lemma LamEq_wf i : wf.t (LamEq i).
-    Proof. crush_wf. Qed.
-
-    (* H >> n1 m1 = n2 m2 in T
-         H >> n1 = n2 in x:A -> B
-         H >> m1 = m2 in A
-         H >> [n1/x]B = T in U(i) *)
-    Definition ApEq (i : nat) (ty : expr.t) : tactic.t :=
-      fun R g =>
-      match g with
-      | H >> expr.Eq (expr.App n1 m1) (expr.App n2 m2) T =>
-        _ <- assume_sb (expr.wf.dec (length H) ty) ;;
-        match ty with
-        | expr.Pi A B =>
-          ret (ternary_derivation (derivation.Ap_Eq i (expr.Pi A B))
-                  (H >> expr.Eq n1 n2 (expr.Pi A B))
-                  (H >> expr.Eq m1 m2 A)
-                  (H >> expr.Eq (expr.subst B 0 n1) T (expr.Uni i)))
-        | _ => fail
-        end
-      | _ => fail
-      end.
-
-    Lemma ApEq_wf i ty : wf.t (ApEq i ty).
-    Proof. crush_wf. Qed.
-
-    (* H >> e1 = e2 in x:A -> B
-           H >> e1 = e1 in x:A -> B
-           H >> e2 = e2 in x:A -> B
-           H, x:A >> e1 x = e2 x in B *)
-    Definition FunExt : tactic.t :=
-      fun R g =>
-      match g with
-      | H >> expr.Eq e1 e2 (expr.Pi A B) =>
-        ret (ternary_derivation derivation.Fun_Ext
-                (H >> expr.Eq e1 e1 (expr.Pi A B))
-                (H >> expr.Eq e2 e2 (expr.Pi A B))
-                (A :: H >> expr.Eq (expr.App (expr.lift 0 1 e1) (expr.Var 0))
-                                   (expr.App (expr.lift 0 1 e2) (expr.Var 0))
-                                   B))
-
-      | _ => fail
-      end.
-
-    Lemma FunExt_wf : wf.t FunExt.
-    Proof. crush_wf. Qed.
-  End pi.
-
-  Module uni.
-    (* H >> U(i) = U(i) in U(i+1) *)
-    Definition Eq : tactic.t :=
-      fun R g =>
-      match g with
-      | H >> expr.Eq (expr.Uni i) (expr.Uni j) (expr.Uni k) =>
-        _ <- assume_sb (Nat.eq_dec i j) ;;
-        _ <- assume_sb (Nat.eq_dec (S i) k) ;;
-        ret (nullary_derivation derivation.Uni_Eq)
-      | _ => fail
-      end.
-
-    Lemma Eq_wf : wf.t Eq.
-    Proof. crush_wf. Qed.
+Definition is_digit (a : Ascii.ascii) : bool := false.
 
 
-    (* H >> A = B in U(i+1)
-         H >> A = B in U(i) *)
-    Definition Cumulative : tactic.t :=
-      fun R g =>
-      match g with
-      | H >> expr.Eq A B (expr.Uni (S i)) =>
-        ret (unary_derivation derivation.Cumulative
-                (H >> expr.Eq A B (expr.Uni i)))
-      | _ => fail
-      end.
+Fixpoint string_to_list s :=
+  match s with
+  | String.EmptyString => nil
+  | String.String c s' => c :: (string_to_list s')
+  end.
 
-    Lemma Cumulative_Eq : wf.t Cumulative.
-    Proof. crush_wf. Qed.
-  End uni.
+Fixpoint list_to_string l :=
+  match l with
+  | nil => String.EmptyString
+  | h::l' => String.String h (list_to_string l')
+  end.
 
-  Module general.
-    (* H >> C
-         H(n) = C *)
-    Definition Hyp (n : nat) : tactic.t :=
-      fun R g =>
-      match g with
-      | H >> C =>
-        ty <- unwrap (telescope.nth H n) ;;
-        _ <- assume_sb (expr.eq_dec C ty) ;;
-        ret (nullary_derivation (derivation.Var n))
-      end.
+Definition nat_to_string (n : nat) : String.string :=
+  list_to_string (List.map decimal_digit_to_ascii (digits 10 n)).
 
-    Lemma Hyp_wf n : wf.t (Hyp n).
-    Proof. crush_wf. Qed.
+(*
+Fixpoint from_digits (base : nat) (l : list nat) : nat :=
+  match l with
+  | [] => 0
+  | d :: l => base * from_digits base l + d
+  end.
 
-    (* H >> x = x in A
-         H(x) = A *)
-    Definition HypEq : tactic.t :=
-      fun R g =>
-      match g with
-      | H >> expr.Eq (expr.Var n1) (expr.Var n2) A =>
-        _ <- assume_sb (Nat.eq_dec n1 n2) ;;
-        ty <- unwrap (telescope.nth H n1) ;;
-        _ <- assume_sb (expr.eq_dec A ty) ;;
-        ret (nullary_derivation derivation.Var_Eq)
-      | _ => fail
-      end.
+Definition nat_from_string (s : String.string) : nat :=
+  from_digits 10 (List.rev (List.map ascii_to_decimal_digit (string_to_list s))).
 
-    Lemma HypEq_wf : wf.t HypEq.
-    Proof. crush_wf. Qed.
-  End general.
+Lemma string_to_list_to_string :
+  forall s, list_to_string (string_to_list s) = s.
+Proof.
+  induction s; auto; simpl.
+  now rewrite IHs.
+Qed.
 
-  Module eq.
-    (* H >>   m1 = n1 in A1   =   m2 = n2 in A2   in U(i)
-           H >> A1 = A2 in U(i)
-           H >> m1 = m2 in A1
-           H >> n1 = n2 in A1 *)
-    Definition Eq : tactic.t :=
-      fun R g =>
-      match g with
-      | H >> expr.Eq (expr.Eq m1 n1 A1) (expr.Eq m2 n2 A2) (expr.Uni i) =>
-        ret (ternary_derivation derivation.Eq_Eq
-                (H >> expr.Eq A1 A2 (expr.Uni i))
-                (H >> expr.Eq m1 m2 A1)
-                (H >> expr.Eq n1 n2 A1))
-      | _ => fail
-      end.
+Lemma list_to_string_to_list :
+  forall l, string_to_list (list_to_string l) = l.
+Proof.
+  induction l; auto; simpl.
+  now rewrite IHl.
+Qed.
 
-    Lemma Eq_wf : wf.t Eq.
-    Proof. crush_wf. Qed.
-  End eq.
-
-  Import expr.exports.
-  Import expr.notations.
-  Local Open Scope expr.
-
-  Module sig.
-    (* H >> x:A * B = x:A' * B' in U(i)
-           H >> A = A' in U(i)
-           H, x:A >> B = B' in U(i) *)
-    Definition Eq : tactic.t :=
-      fun R g =>
-      match g with
-      | H >>  A * B = A' * B' in expr.Uni i =>
-        ret (binary_derivation derivation.Sig_Eq
-               (H >> A = A' in expr.Uni i)
-               (A :: H >> B = B' in expr.Uni i))
-      | _ => fail
-      end.
-
-    Lemma Eq_wf : wf.t Eq.
-    Proof. crush_wf. Qed.
-
-    (* H >> x:A * B
-         H >> a = a in A
-         H >> [a/x]B
-         H, x:A >> B = B in U(i) *)
-    Definition Intro (i : nat) (a : expr.t) : tactic.t :=
-      fun R g =>
-      match g with
-      | H >> A * B =>
-        _ <- assume_sb (expr.wf.dec (length H) a) ;;
-        ret (ternary_derivation (derivation.Sig_Intro i a)
-                (H >> a = a in A)
-                (H >> expr.subst B 0 a)
-                (A :: H >> B = B in Uni i))
-      | _ => fail
-      end.
-
-    Lemma Intro_wf i a : wf.t (Intro i a).
-    Proof. crush_wf. Qed.
-
-    (* H >> C
-         H(n) = x:A * B
-         H, x:A, B >> C *)
-    Definition Elim (n : nat) : tactic.t :=
-      fun R g =>
-      match g with
-      | H >> C =>
-        ty <- unwrap (telescope.nth H n) ;;
-        match ty with
-        | A * B =>
-          ret (unary_derivation (derivation.Sig_Elim n)
-                (B :: A :: H >> expr.lift 0 2 C))
-        | _ => fail
-        end
-      end.
-
-    Lemma Elim_wf n : wf.t (Elim n).
-    Proof. crush_wf. Qed.
-
-    (* H >> (a,b) = (a',b') in x:A * B
-         H >> a = a' in A
-         H >> b = b' in [a/x]B
-         H, x:A >> B = B in U(i) *)
-    Definition PairEq (i : nat) : tactic.t :=
-      fun R g =>
-      match g with
-      | H >> (a,b) = (a',b') in A * B =>
-        ret (ternary_derivation (derivation.Pair_Eq i)
-                (H >> a = a' in A)
-                (H >> b = b' in expr.subst B 0 a)
-                (A :: H >> B = B in Uni i))
-      | _ => fail
-      end.
-
-    Lemma PairEq_wf i : wf.t (PairEq i).
-    Proof. crush_wf. Qed.
-
-    (* H >> fst m1 = fst m2 in A
-         H >> m1 = m2 in A * B
-     *)
-    Definition FstEq (B : expr.t) : tactic.t :=
-      fun R g =>
-      match g with
-      | H >> expr.Fst m1 = expr.Fst m2 in A =>
-        _ <- assume_sb (expr.wf.dec (S (length H)) B) ;;
-        ret (unary_derivation (derivation.Fst_Eq B)
-                (H >> m1 = m2 in A * B))
-      | _ => fail
-      end.
-
-    Lemma FstEq_wf B : wf.t (FstEq B).
-    Proof. crush_wf. Qed.
-
-    (* H >> snd m1 = snd m2 in C
-         H >> m1 = m2 in x:A * B
-         H >> [fst m1/x]B = C in U(i) *)
-    Definition SndEq (i : nat) (ty : expr.t) : tactic.t :=
-      fun R g =>
-      match g with
-      | H >> expr.Snd m1 = expr.Snd m2 in C =>
-        _ <- assume_sb (expr.wf.dec (length H) ty) ;;
-        match ty with
-        | A * B =>
-          ret (binary_derivation (derivation.Snd_Eq i ty)
-                 (H >> m1 = m2 in A * B)
-                 (H >> expr.subst B 0 (Fst m1) = C in Uni i))
-        | _ => fail
-        end
-      | _ => fail
-      end.
+Fixpoint max_suffix (acc : nat) (base : String.string) (l : list String.string) : nat :=
+  match l with
+  | [] => acc
+  | s :: l =>
+    max_suffix
+      (if String.prefix base s
+       then if String.string_dec base s then 1
+            else max (S (S (nat_from_string (String.substring (String.length base) (String.length s) s)))) acc
+       else acc)
+      base
+      l
+  end.
+Open Scope string_scope.
+Eval compute in max_suffix 0 "x" ["xy"].
 
 
-    Lemma SndEq_wf i ty : wf.t (SndEq i ty).
-    Proof. crush_wf. Qed.
-  End sig.
-End rules.
-Import rules.
-
-(* We can use our rules to prove stuff! *)
-Eval compute in refiner.prove (expr.Eq expr.Unit expr.Unit (expr.Uni 0)) rules.unit.Eq.
-Eval compute in refiner.prove expr.Unit rules.unit.Intro.
-Eval compute in refiner.prove (expr.Eq expr.tt expr.tt expr.Unit) rules.unit.TTEq.
+Definition fresh (base : String.string) (l : list String.string) : String.string.
+*)
 
 Module ast.
   (* Okay so it turns out that writing de Bruijn indices by hand is basically
@@ -1135,6 +1167,9 @@ Module ast.
   | Unit : t
 
   | Eq : t -> t -> t -> t
+
+  | Ceq : t -> t -> t
+
   | Uni (level : nat) : t
 
   | Cust : guid.t -> t
@@ -1166,6 +1201,8 @@ Module ast.
     Notation "A * B" := (ast.Sig "_" A B) : ast_scope.
     Notation "A = B 'in' C" := (ast.Eq A B C) (at level 70, B at next level) : ast_scope.
 
+    Notation "A ~ B" := (ast.Ceq A B) (at level 70) : ast_scope.
+
     Local Open Scope ast.
     Import String.
     Local Open Scope string.
@@ -1177,6 +1214,7 @@ Module ast.
     Check ("x", "x").
     Check {"_" : (\ "x", "x")} * (\ "x", "x").
     Check (\ "x", "x") = (\ "x", "x") in Unit.
+    Check (\ "x", "x") ~ (\ "x", "x").
   End notations.
 
 
@@ -1247,6 +1285,12 @@ Module ast.
       match to_expr' l a3 with None => None
       | Some a3 => Some (expr.Eq a1 a2 a3)
       end end end
+    | Ceq a1 a2 =>
+      match to_expr' l a1 with None => None
+      | Some a1 =>
+      match to_expr' l a2 with None => None
+      | Some a2 => Some (expr.Ceq a1 a2)
+      end end
     | Uni i => Some (expr.Uni i)
     | Cust g => Some (expr.Cust g)
     end.
@@ -1254,7 +1298,690 @@ Module ast.
   Fixpoint to_expr (a : t) : option expr.t :=
     to_expr' [] a.
 
+  Fixpoint from_expr' (l : list String.string) (e : expr.t) : option ast.t :=
+    let fresh l := String.append "_" (String.append "x" (nat_to_string (length l))) in
+    match e with
+    | expr.Var n =>
+      match nth_error l n with
+      | Some s => Some (Var s)
+      | None => None
+      end
+    | expr.Lam e =>
+      match from_expr' (fresh l :: l) e with None => None
+      | Some a => Some (Lam (fresh l) a)
+      end
+    | expr.App e1 e2 =>
+      match from_expr' l e1 with None => None
+      | Some a1 =>
+      match from_expr' l e2 with None => None
+      | Some a2 => Some (App a1 a2)
+      end end
+    | expr.Pi e1 e2 =>
+      match from_expr' l e1 with None => None
+      | Some a1 =>
+      match from_expr' (fresh l :: l) e2 with None => None
+      | Some a2 => Some (Pi (fresh l) a1 a2)
+      end end
+    | expr.Pair e1 e2 =>
+      match from_expr' l e1 with None => None
+      | Some a1 =>
+      match from_expr' l e2 with None => None
+      | Some a2 => Some (Pair a1 a2)
+      end end
+    | expr.Fst e =>
+      match from_expr' l e with None => None
+      | Some a => Some (Fst a)
+      end
+    | expr.Snd e =>
+      match from_expr' l e with None => None
+      | Some a => Some (Snd a)
+      end
+    | expr.Sig e1 e2 =>
+      match from_expr' l e1 with None => None
+      | Some a1 =>
+      match from_expr' (fresh l :: l) e2 with None => None
+      | Some a2 => Some (Sig (fresh l) a1 a2)
+      end end
+    | expr.tt => Some tt
+    | expr.Unit => Some Unit
+    | expr.Eq e1 e2 e3 =>
+      match from_expr' l e1 with None => None
+      | Some a1 =>
+      match from_expr' l e2 with None => None
+      | Some a2 =>
+      match from_expr' l e3 with None => None
+      | Some a3 => Some (Eq a1 a2 a3)
+      end end end
+    | expr.Ceq e1 e2 =>
+      match from_expr' l e1 with None => None
+      | Some a1 =>
+      match from_expr' l e2 with None => None
+      | Some a2 => Some (Ceq a1 a2)
+      end end
+    | expr.Uni i => Some (Uni i)
+    | expr.Cust g => Some (Cust g)
+    end.
+
+  Definition from_expr e := from_expr' [] e.
 End ast.
+
+Module rules.
+  Import P.
+  Import tactic_monad.
+  Local Open Scope tactic_monad.
+
+  Import sequent.notations.
+  Local Open Scope sequent.
+
+  Open Scope string_scope.
+
+  Definition nullary_derivation (d : derivation.t) :=
+    tactic_result.Make(G:=sequent.t expr.t) (fun _ => Some d) [].
+
+  Definition unary_derivation (d : derivation.t -> derivation.t) g :=
+    tactic_result.Make(G:=sequent.t expr.t) (fun l => match l with
+                                            | [x]  => Some (d x)
+                                            | _ => None
+                                            end) [g].
+
+  Definition binary_derivation (d : derivation.t -> derivation.t -> derivation.t) g1 g2 :=
+    tactic_result.Make(G:=sequent.t expr.t)
+      (fun l => match l with
+             | [d1; d2] => Some (d d1 d2)
+             | _ => None
+             end)
+      [g1; g2].
+
+  Definition ternary_derivation (d : derivation.t -> derivation.t ->
+                                     derivation.t -> derivation.t) g1 g2 g3 :=
+    tactic_result.Make(G:=sequent.t expr.t)
+      (fun l => match l with
+             | [d1; d2; d3] => Some (d d1 d2 d3)
+             | _ => None
+             end)
+      [g1; g2; g3].
+
+  Module wf.
+    Definition t (rule : tactic.t) : Prop :=
+      forall g res,
+        sequent.wf.t g ->
+        run (rule _ g) = Some res ->
+        tactic_result.wf.t (fun g d => derivation.wf.t (length (sequent.context g)) d) g res /\
+        List.Forall sequent.wf.t (tactic_result.goals res).
+  End wf.
+
+  Ltac head_symbol e :=
+    match e with
+    | ?f ?x => head_symbol f
+    | _ => e
+    end.
+
+  Ltac crush_wf :=
+    match goal with
+    | [ |- wf.t ?f ] => let x := head_symbol f in unfold x
+    end;
+    unfold wf.t;
+    intros;
+    unfold_tactic_monad;
+    repeat break_match; try discriminate;
+    find_inversion;
+    unfold nullary_derivation, unary_derivation, binary_derivation, ternary_derivation;
+    simpl in *; repeat break_and; split; [
+      unfold tactic_result.wf.t; simpl; intros;
+      repeat match goal with
+             | [ H : Forall2 _ _ _ |- _ ] => invc H
+             end;
+      eexists; intuition eauto; simpl in *; intuition;
+      eauto using telescope.nth_length
+    | unfold sequent.wf.t in *;
+      repeat (apply Forall_cons || apply Forall_nil); simpl; intuition;
+      try match goal with
+      | [ H : telescope.nth _ _ = Some _ |- expr.wf.t _ _ ] =>
+        eapply telescope.wf.nth in H; [|solve[eauto]]; simpl in H; intuition
+      end ];
+    auto using expr.wf.subst with arith;
+    try match goal with
+    | [  |- expr.wf.t _ (expr.lift _ ?n _) ] =>
+      solve [apply expr.wf.lift' with (d := n); auto]
+    end.
+
+  Module unit.
+    (* H >> unit = unit in U(i) *)
+    Definition Eq : tactic.t :=
+      fun R g =>
+      match g with
+      | H >> (expr.Eq expr.Unit expr.Unit (expr.Uni _)) =>
+        ret (nullary_derivation derivation.Unit_Eq)
+      | _ => fail
+      end.
+
+    Lemma Eq_wf : wf.t Eq.
+    Proof. crush_wf. Qed.
+
+    (* H >> unit *)
+    Definition Intro : tactic.t :=
+      fun R g =>
+      match g with
+      | H >> expr.Unit => ret (nullary_derivation derivation.Unit_Intro)
+      | _ => fail
+      end.
+
+    Lemma Intro_wf : wf.t Intro.
+    Proof. crush_wf. Qed.
+
+    (* H >> tt = tt in unit *)
+    Definition TTEq : tactic.t :=
+      fun R g =>
+      match g with
+      | H >> (expr.Eq expr.tt expr.tt expr.Unit) =>
+        ret (nullary_derivation derivation.tt_Eq)
+      | _ => fail
+      end.
+
+    Lemma TTEq_wf : wf.t TTEq.
+    Proof. crush_wf. Qed.
+  End unit.
+
+  Module pi.
+    (* H >> x:A -> B = x:A' -> B' in U(i)
+         H >> A = A' in U(i)
+         H, x:A >> B = B' in U(i) *)
+    Definition Eq x : tactic.t :=
+      fun R g =>
+      match g with
+      | H >> expr.Eq (expr.Pi A B) (expr.Pi A' B') (expr.Uni i) =>
+        ret (binary_derivation derivation.Pi_Eq
+                (H >> (expr.Eq A A' (expr.Uni i)))
+                ((x, A) :: H >> (expr.Eq B B' (expr.Uni i))))
+      | _ => fail
+      end.
+
+    Lemma Eq_wf x : wf.t (Eq x).
+    Proof. crush_wf. Qed.
+
+    (* H >> x:A -> B
+         H >> A = A in U(i)
+         H, x:A >> B *)
+    Definition Intro (i : nat) x : tactic.t :=
+      fun R g =>
+      match g with
+      | H >> expr.Pi A B =>
+        ret (binary_derivation (derivation.Pi_Intro i)
+                (H >> expr.Eq A A (expr.Uni i))
+                ((x, A) :: H >> B))
+      | _ => fail
+      end.
+
+    Lemma Intro_wf i x : wf.t (Intro i x).
+    Proof. crush_wf. Qed.
+
+    (* H >> C
+         H(n) = x:A -> B
+         H >> e = e in A
+         H, [e/x]B >> C
+     *)
+    Definition Elim (n : nat) (a : ast.t) x : tactic.t :=
+      fun R g =>
+      match g with
+      | H >> C =>
+        e <- unwrap (ast.to_expr' (telescope.names H) a) ;;
+        _ <- assume_sb (expr.wf.dec (length H) e) ;;
+        ty <- unwrap (telescope.nth H n) ;;
+        match ty with
+        | expr.Pi A B =>
+          ret (binary_derivation (derivation.Pi_Elim n e)
+                  (H >> expr.Eq e e A)
+                  ((x, expr.subst B 0 e) :: H >> expr.lift 0 1 C))
+        | _ => fail
+        end
+      end.
+
+    Lemma Elim_wf n e x : wf.t (Elim n e x).
+    Proof. crush_wf. Qed.
+
+    (* H >> \x.e = \x.e' in x:A -> B
+         H >> A = A in U(i)
+         H, x:A >> e = e' in B *)
+    Definition LamEq (i : nat) x : tactic.t :=
+      fun R g =>
+      match g with
+      | H >> expr.Eq (expr.Lam e) (expr.Lam e') (expr.Pi A B) =>
+        ret (binary_derivation (derivation.Lam_Eq i)
+                (H >> expr.Eq A A (expr.Uni i))
+                ((x, A) :: H >> expr.Eq e e' B))
+      | _ => fail
+      end.
+
+    Lemma LamEq_wf i x : wf.t (LamEq i x).
+    Proof. crush_wf. Qed.
+
+    (* H >> n1 m1 = n2 m2 in T
+         H >> n1 = n2 in x:A -> B
+         H >> m1 = m2 in A
+         H >> [n1/x]B = T in U(i) *)
+    Definition ApEq (i : nat) (ty_a : ast.t) : tactic.t :=
+      fun R g =>
+      match g with
+      | H >> expr.Eq (expr.App n1 m1) (expr.App n2 m2) T =>
+        ty <- unwrap (ast.to_expr' (telescope.names H) ty_a) ;;
+        _ <- assume_sb (expr.wf.dec (length H) ty) ;;
+        match ty with
+        | expr.Pi A B =>
+          ret (ternary_derivation (derivation.Ap_Eq i (expr.Pi A B))
+                  (H >> expr.Eq n1 n2 (expr.Pi A B))
+                  (H >> expr.Eq m1 m2 A)
+                  (H >> expr.Eq (expr.subst B 0 n1) T (expr.Uni i)))
+        | _ => fail
+        end
+      | _ => fail
+      end.
+
+    Lemma ApEq_wf i ty : wf.t (ApEq i ty).
+    Proof. crush_wf. Qed.
+
+    (* H >> e1 = e2 in x:A -> B
+           H >> e1 = e1 in x:A -> B
+           H >> e2 = e2 in x:A -> B
+           H, x:A >> e1 x = e2 x in B *)
+    Definition FunExt x : tactic.t :=
+      fun R g =>
+      match g with
+      | H >> expr.Eq e1 e2 (expr.Pi A B) =>
+        ret (ternary_derivation derivation.Fun_Ext
+                (H >> expr.Eq e1 e1 (expr.Pi A B))
+                (H >> expr.Eq e2 e2 (expr.Pi A B))
+                ((x, A) :: H >> expr.Eq (expr.App (expr.lift 0 1 e1) (expr.Var 0))
+                                   (expr.App (expr.lift 0 1 e2) (expr.Var 0))
+                                   B))
+
+      | _ => fail
+      end.
+
+    Lemma FunExt_wf x : wf.t (FunExt x).
+    Proof. crush_wf. Qed.
+  End pi.
+
+  Module uni.
+    (* H >> U(i) = U(i) in U(i+1) *)
+    Definition Eq : tactic.t :=
+      fun R g =>
+      match g with
+      | H >> expr.Eq (expr.Uni i) (expr.Uni j) (expr.Uni k) =>
+        _ <- assume_sb (Nat.eq_dec i j) ;;
+        _ <- assume_sb (Nat.eq_dec (S i) k) ;;
+        ret (nullary_derivation derivation.Uni_Eq)
+      | _ => fail
+      end.
+
+    Lemma Eq_wf : wf.t Eq.
+    Proof. crush_wf. Qed.
+
+
+    (* H >> A = B in U(i+1)
+         H >> A = B in U(i) *)
+    Definition Cumulative : tactic.t :=
+      fun R g =>
+      match g with
+      | H >> expr.Eq A B (expr.Uni (S i)) =>
+        ret (unary_derivation derivation.Cumulative
+                (H >> expr.Eq A B (expr.Uni i)))
+      | _ => fail
+      end.
+
+    Lemma Cumulative_Eq : wf.t Cumulative.
+    Proof. crush_wf. Qed.
+  End uni.
+
+  Import expr.exports.
+  Import expr.notations.
+  Local Open Scope expr.
+
+  Module general.
+    (* H >> C
+         H(n) = C *)
+    Definition Hyp (n : nat) : tactic.t :=
+      fun R g =>
+      match g with
+      | H >> C =>
+        ty <- unwrap (telescope.nth H n) ;;
+        _ <- assume_sb (expr.eq_dec C ty) ;;
+        ret (nullary_derivation (derivation.Var n))
+      end.
+
+    Lemma Hyp_wf n : wf.t (Hyp n).
+    Proof. crush_wf. Qed.
+
+    (* H >> x = x in A
+         H(x) = A *)
+    Definition HypEq : tactic.t :=
+      fun R g =>
+      match g with
+      | H >> expr.Var n1 = expr.Var n2 in A =>
+        _ <- assume_sb (Nat.eq_dec n1 n2) ;;
+        ty <- unwrap (telescope.nth H n1) ;;
+        _ <- assume_sb (expr.eq_dec A ty) ;;
+        ret (nullary_derivation derivation.Var_Eq)
+      | _ => fail
+      end.
+
+    Lemma HypEq_wf : wf.t HypEq.
+    Proof. crush_wf. Qed.
+
+    Definition Witness (a : ast.t) : tactic.t :=
+      fun R g =>
+      match g with
+      | H >> C =>
+        e <- unwrap (ast.to_expr' (telescope.names H) a) ;;
+        _ <- assume_sb (expr.wf.dec (length H) e) ;;
+        ret (unary_derivation (derivation.Witness e)
+              (H >> e = e in C))
+      end.
+
+    Lemma Witness_wf a : wf.t (Witness a).
+    Proof. crush_wf. Qed.
+
+    Definition Compute (n : nat) : tactic.t :=
+      fun R g =>
+      match g with
+      | H >> C =>
+        C' <- unwrap (run.f n C) ;;
+        ret (unary_derivation (fun x => x)
+              (H >> C'))
+      end.
+
+    Lemma Compute_wf n : wf.t (Compute n).
+    Proof. crush_wf. Admitted.
+  End general.
+
+  Module eq.
+    (* H >>   m1 = n1 in A1   =   m2 = n2 in A2   in U(i)
+           H >> A1 = A2 in U(i)
+           H >> m1 = m2 in A1
+           H >> n1 = n2 in A1 *)
+    Definition Eq : tactic.t :=
+      fun R g =>
+      match g with
+      | H >> (m1 = n1 in A1) = (m2 = n2 in A2) in expr.Uni i =>
+        ret (ternary_derivation derivation.Eq_Eq
+                (H >> A1 = A2 in expr.Uni i)
+                (H >> m1 = m2 in A1)
+                (H >> n1 = n2 in A1))
+      | _ => fail
+      end.
+
+    Lemma Eq_wf : wf.t Eq.
+    Proof. crush_wf. Qed.
+  End eq.
+
+  Module sig.
+    (* H >> x:A * B = x:A' * B' in U(i)
+           H >> A = A' in U(i)
+           H, x:A >> B = B' in U(i) *)
+    Definition Eq (x : String.string) : tactic.t :=
+      fun R g =>
+      match g with
+      | H >>  A * B = A' * B' in expr.Uni i =>
+        ret (binary_derivation derivation.Sig_Eq
+               (H >> A = A' in expr.Uni i)
+               ((x, A)%core :: H >> B = B' in expr.Uni i))
+      | _ => fail
+      end.
+
+    Lemma Eq_wf x : wf.t (Eq x).
+    Proof. crush_wf. Qed.
+
+    (* H >> x:A * B
+         H >> a = a in A
+         H >> [a/x]B
+         H, x:A >> B = B in U(i) *)
+    Definition Intro (i : nat) (a : ast.t) x : tactic.t :=
+      fun R g =>
+      match g with
+      | H >> A * B =>
+        e <- unwrap (ast.to_expr' (telescope.names H) a) ;;
+        _ <- assume_sb (expr.wf.dec (length H) e) ;;
+        ret (ternary_derivation (derivation.Sig_Intro i e)
+                (H >> e = e in A)
+                (H >> expr.subst B 0 e)
+                ((x,A)%core :: H >> B = B in Uni i))
+      | _ => fail
+      end.
+
+    Lemma Intro_wf i a x : wf.t (Intro i a x).
+    Proof. crush_wf. Qed.
+
+    (* H >> C
+         H(n) = x:A * B
+         H, x:A, B >> C *)
+    Definition Elim (n : nat) x y : tactic.t :=
+      fun R g =>
+      match g with
+      | H >> C =>
+        ty <- unwrap (telescope.nth H n) ;;
+        match ty with
+        | A * B =>
+          ret (unary_derivation (derivation.Sig_Elim n)
+                ((y,B) :: (x,A) :: H >> expr.lift 0 2 C)%core)
+        | _ => fail
+        end
+      end.
+
+    Lemma Elim_wf n x y : wf.t (Elim n x y ).
+    Proof. crush_wf. Qed.
+
+    (* H1, z : x:A * B, H2 >> C
+         H1, z : x:A * B, a:A, b:[a/x]B, [(a,b)/z]H2 >> [(a,b)/z] C *)
+    Definition Elim' (a : ast.t) x y : tactic.t :=
+      fun R g =>
+      match g with
+      | H >> C =>
+        e <- unwrap (ast.to_expr' (telescope.names H) a);;
+        match e with
+        | expr.Var n =>
+          ty <- unwrap (telescope.nth H n) ;;
+          match telescope.split H n with
+          | Some (H1, (_, A * B), H2)%core =>
+            let H1 := telescope.lift (S n) 2 H1 in
+            let C := expr.lift (S n) 2 C in
+            let H := telescope.subst H1 n (S n, n) ++ (y,B) :: (x,A) :: H2 in
+            let C := expr.subst C n (S n, n) in
+
+            ret (unary_derivation (derivation.Sig_Elim n)
+                  (H >> C))
+          | _ => fail
+          end%core
+        | _ => fail
+        end
+      end.
+
+(*
+          ret (unary_derivation (derivation.Sig_Elim n)
+                (B :: A :: H1 >> expr.lift (length H1) 2 C)) *)
+
+    Lemma Elim'_wf n x y : wf.t (Elim' n x y).
+    Proof. crush_wf. Admitted.
+
+    (* H >> (a,b) = (a',b') in x:A * B
+         H >> a = a' in A
+         H >> b = b' in [a/x]B
+         H, x:A >> B = B in U(i) *)
+    Definition PairEq (i : nat) x : tactic.t :=
+      fun R g =>
+      match g with
+      | H >> (a,b) = (a',b') in A * B =>
+        ret (ternary_derivation (derivation.Pair_Eq i)
+                (H >> a = a' in A)
+                (H >> b = b' in expr.subst B 0 a)
+                ((x,A)%core :: H >> B = B in Uni i))
+      | _ => fail
+      end.
+
+    Lemma PairEq_wf i x : wf.t (PairEq i x).
+    Proof. crush_wf. Qed.
+
+    (* H >> fst m1 = fst m2 in A
+         H >> m1 = m2 in A * B
+     *)
+    Definition FstEq (B_a : ast.t) : tactic.t :=
+      fun R g =>
+      match g with
+      | H >> expr.Fst m1 = expr.Fst m2 in A =>
+        B <- unwrap (ast.to_expr' (telescope.names H) B_a) ;;
+        _ <- assume_sb (expr.wf.dec (S (length H)) B) ;;
+        ret (unary_derivation (derivation.Fst_Eq B)
+                (H >> m1 = m2 in A * B))
+      | _ => fail
+      end.
+
+    Lemma FstEq_wf B : wf.t (FstEq B).
+    Proof. crush_wf. Qed.
+
+    (* H >> snd m1 = snd m2 in C
+         H >> m1 = m2 in x:A * B
+         H >> [fst m1/x]B = C in U(i) *)
+    Definition SndEq (i : nat) (ty_a : ast.t) : tactic.t :=
+      fun R g =>
+      match g with
+      | H >> expr.Snd m1 = expr.Snd m2 in C =>
+        ty <- unwrap (ast.to_expr' (telescope.names H) ty_a) ;;
+        _ <- assume_sb (expr.wf.dec (length H) ty) ;;
+        match ty with
+        | A * B =>
+          ret (binary_derivation (derivation.Snd_Eq i ty)
+                 (H >> m1 = m2 in A * B)
+                 (H >> expr.subst B 0 (Fst m1) = C in Uni i))
+        | _ => fail
+        end
+      | _ => fail
+      end.
+
+    Lemma SndEq_wf i ty : wf.t (SndEq i ty).
+    Proof. crush_wf. Qed.
+  End sig.
+
+  Module ceq.
+    (* H >> a ~ a *)
+    Definition Refl : tactic.t :=
+      fun R g =>
+      match g with
+      | H >> e1 ~ e2 =>
+        _ <- assume_sb (expr.eq_dec e1 e2) ;;
+        ret (nullary_derivation derivation.Ceq_Refl)
+      | _ => fail
+      end.
+
+    Lemma Refl_wf : wf.t Refl.
+    Proof. crush_wf. Qed.
+
+    Definition Sym : tactic.t :=
+      fun R g =>
+      match g with
+      | H >> e1 ~ e2 =>
+        ret (unary_derivation derivation.Ceq_Sym
+              (H >> e2 ~ e1))
+      | _ => fail
+      end.
+
+    Lemma Sym_wf : wf.t Sym.
+    Proof. crush_wf. Qed.
+
+    Definition Mem_Eq : tactic.t :=
+      fun R g =>
+      match g with
+      | H >> expr.tt = expr.tt in (e1 ~ e2) =>
+        ret (unary_derivation derivation.Ceq_Mem_Eq
+              (H >> e1 ~ e2))
+      | _ => fail
+      end.
+
+    Lemma Mem_Eq_wf : wf.t Mem_Eq.
+    Proof. crush_wf. Qed.
+
+    Definition Eq : tactic.t :=
+      fun R g =>
+      match g with
+      | H >> (e1 ~ e2) = (e3 ~ e4) in expr.Uni i =>
+        ret (binary_derivation derivation.Ceq_Eq
+              (H >> e1 ~ e3)
+              (H >> e2 ~ e4))
+      | _ => fail
+      end.
+
+    Lemma Eq_wf : wf.t Eq.
+    Proof. crush_wf. Qed.
+
+    Definition Step : tactic.t :=
+      fun R g =>
+      match g with
+      | H >> e1 ~ e2 =>
+        match step.f e1 with
+        | step.result.Step e1' =>
+          ret (unary_derivation derivation.Ceq_Step
+                (H >> e1' ~ e2))
+        | _ => fail
+        end
+      | _ => fail
+      end.
+
+    Lemma Step_wf : wf.t Step.
+    Proof. crush_wf. Admitted.
+
+    Definition Subst (x : String.string) (ty_a : ast.t) (C_a : ast.t) : tactic.t :=
+      fun R g =>
+      match g with
+      | H >> Ca =>
+        ty <- unwrap (ast.to_expr' (telescope.names H) ty_a) ;;
+        _ <- assume_sb (expr.wf.dec (length H) ty) ;;
+
+        match ty with
+        | a ~ b =>
+          C <- unwrap (ast.to_expr' (x :: telescope.names H) C_a) ;;
+          _ <- assume_sb (expr.wf.dec (S (length H)) C) ;;
+          _ <- assume_sb (expr.eq_dec Ca (expr.subst C 0 a)) ;;
+          ret (binary_derivation (derivation.Ceq_Subst C)
+                 (H >> a ~ b)
+                 (H >> expr.subst C 0 b))
+        | _ => fail
+        end
+      end.
+
+    Lemma Subst_wf x ty_a C_a : wf.t (Subst x ty_a C_a).
+    Proof. crush_wf. Qed.
+  End ceq.
+End rules.
+Import rules.
+
+(* We can use our rules to prove stuff! *)
+Eval compute in refiner.prove (expr.Eq expr.Unit expr.Unit (expr.Uni 0)) rules.unit.Eq.
+Eval compute in refiner.prove expr.Unit rules.unit.Intro.
+Eval compute in refiner.prove (expr.Eq expr.tt expr.tt expr.Unit) rules.unit.TTEq.
+
+Fixpoint unparse_telescope' (l : list String.string) (C : outermost_first_telescope.t expr.t) : option (outermost_first_telescope.t ast.t) :=
+  match C with
+  | [] => Some []
+  | (n,e) :: C =>
+    match ast.from_expr' l e with
+    | None => None
+    | Some a =>
+      match unparse_telescope' (n :: l) C with
+      | None => None
+      | Some C => Some ((n, a) :: C)
+      end
+    end
+  end.
+
+Definition unparse_sequent (s : sequent.t expr.t) : option (sequent.t ast.t) :=
+  match s with
+  | sequent.Make H C =>
+    match unparse_telescope' [] (telescope.to_outer H) with
+    | None => None
+    | Some H' =>
+      match ast.from_expr' (telescope.names H) C with
+      | None => None
+      | Some C => Some (sequent.Make H' C)
+      end
+    end
+  end.
 
 Open Scope string_scope.
 
@@ -1299,6 +2026,8 @@ Ltac parse' l e :=
    extensionality without copy-pasting. *)
 Definition funext : expr.t := ltac:(parse ast_funext).
 
+Eval compute in ast.from_expr funext.
+
 (* A few simple notations for the tactics. *)
 Notation "t ;; l" := (P.split t l) (at level 50, left associativity).
 Notation "t1 ;;; t2" := (P.next t1 t2) (at level 50, left associativity).
@@ -1308,24 +2037,28 @@ Module tac_info.
   Record t :=
     Make {
         i : option nat;
-        e : option expr.t
+        a : option ast.t;
+        ns : list String.string
       }.
 
-  Definition empty : t := Make None None.
-  Definition level (i : nat) : t := Make (Some i) None.
-  Definition arg (e : expr.t) : t := Make None (Some e).
+  Definition empty : t := Make None None [].
+  Definition level (i : nat) : t := Make (Some i) None [].
+  Definition arg (a : ast.t) : t := Make None (Some a) [].
+  Definition names l : t := Make None None l.
 
   Definition get_i (x : t) {R} : tactic_monad.t R nat :=
-    match i x with
-    | Some i => tactic_monad.ret i
-    | None => tactic_monad.fail
-    end.
+    tactic_monad.unwrap (i x).
 
-  Definition get_e (x : t) {R} : tactic_monad.t R expr.t :=
-    match e x with
-    | Some e => tactic_monad.ret e
-    | None => tactic_monad.fail
-    end.
+  Definition get_a (x : t) {R} : tactic_monad.t R ast.t :=
+    tactic_monad.unwrap (a x).
+
+  Definition get_ith_name' (x : t) (i : nat) {R} : tactic_monad.t R String.string :=
+    tactic_monad.unwrap (nth_error (ns x) i).
+
+  Definition get_ith_name (x : t) (i : nat) {R} : tactic_monad.t R String.string :=
+    tactic_monad.choose [fun _ => get_ith_name' x i; fun _ => tactic_monad.ret "x"].
+
+  Definition get_name (x : t) {R} := get_ith_name(R := R) x 0.
 End tac_info.
 
 Module tac.
@@ -1333,23 +2066,31 @@ Module tac.
     refine (fun R g => _).
     refine (tactic_monad.choose
               [fun _ => unit.Intro g;
-               fun _ => tactic_monad.bind (tac_info.get_i info) (fun i => pi.Intro i g);
                fun _ => tactic_monad.bind (tac_info.get_i info) (fun i =>
-                     tactic_monad.bind (tac_info.get_e info) (fun e => sig.Intro i e g))]).
+                     tactic_monad.bind (tac_info.get_name info) (fun x =>
+                     pi.Intro i x g));
+               fun _ => tactic_monad.bind (tac_info.get_i info) (fun i =>
+                     tactic_monad.bind (tac_info.get_a info) (fun e =>
+                     tactic_monad.bind (tac_info.get_name info) (fun x =>
+                     sig.Intro i e x g)))]).
   Defined.
 
   Definition Eq (info : tac_info.t) : tactic.t.
     refine (fun R g => _).
     refine (tactic_monad.choose
               [fun _ => unit.Eq g;
-               fun _ => pi.Eq g;
-               fun _ => sig.Eq g;
+               fun _ => tactic_monad.bind (tac_info.get_name info) (fun x => pi.Eq x g);
+               fun _ => tactic_monad.bind (tac_info.get_name info) (fun x => sig.Eq x g);
                fun _ => uni.Eq g;
                fun _ => eq.Eq g;
                fun _ => unit.TTEq g;
                fun _ => general.HypEq g;
-               fun _ => tactic_monad.bind (tac_info.get_i info) (fun i => pi.LamEq i g);
-               fun _ => tactic_monad.bind (tac_info.get_i info) (fun i => sig.PairEq i g)
+               fun _ => tactic_monad.bind (tac_info.get_i info) (fun i =>
+                     tactic_monad.bind (tac_info.get_name info) (fun x =>
+                     pi.LamEq i x g));
+               fun _ => tactic_monad.bind (tac_info.get_i info) (fun i =>
+                     tactic_monad.bind (tac_info.get_name info) (fun x =>
+                     sig.PairEq i x g))
            ]).
   Defined.
 
@@ -1369,30 +2110,32 @@ Module tac.
   Defined.
 End tac.
 
+Definition goggles (r : refiner.result.t) : option (list (sequent.t ast.t)) :=
+  match r with
+  | refiner.result.Incomplete l =>
+    sequence_option (List.map unparse_sequent l)
+  | _ => None
+  end.
+
+
 Import sequent.notations.
 Open Scope sequent.
+Open Scope ast.
 
 (* Let's prove function extensionality! *)
 Eval cbv in
   let go_eq := P.repeat 10 (tac.Eq tac_info.empty) in
   refiner.prove funext
-                (pi.Intro 1 ;;; go_eq ;;;
-                 pi.Intro 1 ;;; go_eq ;;;
-                 pi.Intro 0 ;;; go_eq ;;;
-                 pi.Intro 0 ;;; go_eq ;;;
-                 pi.Intro 0 ;;; go_eq ;; [
-                        pi.ApEq 0
-                           (ltac:(parse' ["x"; "g"; "f"; "B"; "A"]
-                                                    (ast.Pi "_" "A" "B")));;; go_eq;
-                        pi.ApEq 0
-                           (ltac:(parse' ["x"; "g"; "f"; "B"; "A"]
-                                                    (ast.Pi "_" "A" "B")));;; go_eq;
-
-                        pi.FunExt;;; go_eq ;;;
-                        pi.Elim 1
-                          (ltac:(parse' ["x"; "H"; "g"; "f"; "B"; "A"] "x"));;;
-                          go_eq;;;
-                        tac.Assumption]).
+                (pi.Intro 1 "A" ;;; go_eq ;;;
+                 pi.Intro 1 "B" ;;; go_eq ;;;
+                 pi.Intro 0 "f" ;;; go_eq ;;;
+                 pi.Intro 0 "g" ;;; go_eq ;;;
+                 pi.Intro 0 "H" ;;; go_eq ;; [
+                     pi.ApEq 0 ("A" -> "B");;; go_eq;
+                     pi.ApEq 0 ("A" -> "B");;; go_eq;
+                     pi.FunExt "x";;; go_eq ;;;
+                     pi.Elim 1 "x" "Hx";;; go_eq ;;;
+                     tac.Assumption]).
 
 Definition ast_proj1 : ast.t :=
   {"A" : Uni 0} ->
@@ -1402,25 +2145,50 @@ Definition ast_proj1 : ast.t :=
 
 Definition proj1 : expr.t := ltac:(parse ast_proj1).
 
-Eval cbv in refiner.prove proj1
-  (pi.Intro 1;; [uni.Eq;
-   pi.Intro 1;; [pi.Eq;; [uni.Cumulative;;; general.HypEq; uni.Eq];
-   pi.Intro 0;; [sig.Eq;; [general.HypEq;
-       pi.ApEq 1
-         (ltac:(parse' ["x"; "B"; "A"] (ast.Pi "y" "A" (ast.Uni 0))));;
-       [general.HypEq; general.HypEq; uni.Eq]];
-   sig.Elim 0;; [general.Hyp 1]]]]).
-
+Eval cbv in
+  let go_eq := P.repeat 10 (tac.Eq tac_info.empty) in
+  refiner.prove proj1
+  (pi.Intro 1 "A" ;;; go_eq ;;;
+   pi.Intro 1 "B" ;; [go_eq ;;; uni.Cumulative;;; general.HypEq; P.id] ;;;
+   pi.Intro 0 "p" ;; [go_eq ;;; pi.ApEq 1 ("A" -> Uni 0);;; go_eq; P.id] ;;;
+   sig.Elim 0 "a" "b" ;;;
+   general.Witness "a" ;;; go_eq).
 
 Definition ast_snd_eq : ast.t :=
   Snd (tt, tt) = Snd (tt, tt) in Unit.
 
 Definition snd_eq : expr.t := ltac:(parse ast_snd_eq).
 
-Eval cbv in refiner.prove snd_eq
-   (sig.SndEq 0 (ltac:(parse (ast.Sig "_" ast.Unit ast.Unit))) ;;
-     [sig.PairEq 0 ;; [unit.TTEq; unit.TTEq; unit.Eq];
-      unit.Eq]).
+Eval cbv in
+  let go_eq := P.repeat 10 (tac.Eq tac_info.empty) in
+    refiner.prove snd_eq
+    (sig.SndEq 0 (Unit * Unit) ;;; go_eq ;;;
+     sig.PairEq 0 "a" ;;; go_eq).
+
+
+Definition ast_pair_eta : ast.t :=
+  {"A" : Uni 0} ->
+  {"B" : "A" -> Uni 0} ->
+  {"z" : ({"x" : "A"} * "B" "x")} ->
+  "z" = (Fst "z", Snd "z") in ({"x" : "A"} * "B" "x").
+
+Definition pair_eta : expr.t := ltac:(parse ast_pair_eta).
+
+Eval cbv in
+  let go_eq := P.repeat 10 (tac.Eq tac_info.empty) in
+  refiner.prove pair_eta
+     (pi.Intro 1 "A" ;;; go_eq ;;;
+      pi.Intro 1 "B" ;;; go_eq ;; [uni.Cumulative;;; go_eq ; P.id];;;
+      pi.Intro 0 "z" ;;; go_eq ;; [pi.ApEq 1 ("A" -> Uni 0);;; go_eq; P.id];;;
+      sig.Elim' "z" "a" "b" ;;;
+      ceq.Subst "x" (Fst ("a", "b") ~ "a")
+                (("a", "b") = ("x", Snd ("a", "b")) in {"_x4" : "A"}* "B" "_x4") ;;
+      [ceq.Step;;; ceq.Refl; P.id];;;
+      ceq.Subst "x" (Snd ("a", "b") ~ "b")
+                (("a", "b") = ("a", "x") in {"_x4" : "A"}* "B" "_x4") ;;
+      [ceq.Step;;; ceq.Refl; P.id];;;
+      sig.PairEq 0 "y";;; go_eq ;;;
+      pi.ApEq 1 ("A" -> Uni 0);;; go_eq).
 
 (* End of main development. *)
 
@@ -1433,8 +2201,8 @@ Module configuration.
   Module entry.
     Record t :=
       Make {
-          type : expr.t 0;
-          extract : expr.t 0
+          type : expr.t;
+          extract : expr.t
         }.
   End entry.
 
@@ -1442,13 +2210,13 @@ Module configuration.
 
   Definition empty : t := []%list.
 
-  Definition insert (name : guid.t) (type : expr.t 0) (extract : expr.t 0) (C : t) : t :=
+  Definition insert (name : guid.t) (type : expr.t) (extract : expr.t) (C : t) : t :=
     assoc_set guid.eq_dec C name (entry.Make type extract).
 
-  Definition type_of (name : guid.t) (C : t) : option (expr.t 0) :=
+  Definition type_of (name : guid.t) (C : t) : option (expr.t) :=
     option_map entry.type (assoc guid.eq_dec C name).
 
-  Definition extract_of (name : guid.t) (C : t) : option (expr.t 0) :=
+  Definition extract_of (name : guid.t) (C : t) : option (expr.t) :=
     option_map entry.extract (assoc guid.eq_dec C name).
 End configuration.
 
@@ -1456,107 +2224,3 @@ End configuration.
 (* Eventually we should give meaning to the proof theory in terms of the
    underlying computation system. Then we should be able to show that the
    rules above are sound. *)
-
-Module value.
-  Inductive t : expr.t 0 -> Prop :=
-  | Lam : forall e, t (expr.Lam e)
-  | Pi : forall e1 e2, t (expr.Pi e1 e2)
-  | tt : t expr.tt
-  | Unit : t expr.Unit
-  | Eq : forall e1 e2 e3, t (expr.Eq e1 e2 e3)
-  | Uni : forall i, t (expr.Uni i)
-  | Cust : forall g, t (expr.Cust g)
-  .
-  Hint Constructors t.
-End value.
-
-Module step.
-  Module result.
-    Inductive t :=
-    | Step : expr.t 0 -> t
-    | Value : t
-    | Stuck : t
-    .
-  End result.
-
-  Inductive t : expr.t 0 -> expr.t 0 -> Prop :=
-  | Beta : forall e1 e2, t (expr.App (expr.Lam e1) e2) (expr.subst e1 [e2])
-  | AppL : forall e1 e1' e2, t e1 e1' -> t (expr.App e1 e2) (expr.App e1' e2)
-  .
-  Hint Constructors t.
-
-  Lemma det : forall e e1 e2, t e e1 -> t e e2 -> e1 = e2.
-  Proof.
-    intros.
-    generalize dependent e2.
-    induction H; intros.
-    - invc H0.
-      + apply Eqdep_dec.inj_pair2_eq_dec in H1; auto using PeanoNat.Nat.eq_dec.
-        apply Eqdep_dec.inj_pair2_eq_dec in H2; auto using PeanoNat.Nat.eq_dec.
-        subst.
-        auto.
-      + apply Eqdep_dec.inj_pair2_eq_dec in H; auto using PeanoNat.Nat.eq_dec.
-        subst.
-        solve_by_inversion.
-    - invc H0.
-      + apply Eqdep_dec.inj_pair2_eq_dec in H2; auto using PeanoNat.Nat.eq_dec.
-        subst.
-        solve_by_inversion.
-      + apply Eqdep_dec.inj_pair2_eq_dec in H1; auto using PeanoNat.Nat.eq_dec.
-        apply Eqdep_dec.inj_pair2_eq_dec in H3; auto using PeanoNat.Nat.eq_dec.
-        subst.
-        f_equal; auto.
-  Qed.
-
-  Definition f (e : expr.t 0) : result.t :=
-    expr.rec0
-      (fun _ => result.t)
-      (* Lam *) (fun _ => result.Value)
-      (* App *) (fun e1 e2 IHe1 _ =>
-                   match IHe1 with
-                   | result.Step e1' => result.Step (expr.App e1' e2)
-                   | result.Value => expr.case0
-                                      _
-                                      (* Lam *)(fun e1 => result.Step (expr.subst e1 [e2]))
-                                      (* App *) (fun _ _ => result.Stuck)
-                                      (* Pi *) (fun _ _ => result.Stuck)
-                                      (* tt *) result.Stuck
-                                      (* Unit *) result.Stuck
-                                      (* Eq *) (fun _ _ _ => result.Stuck)
-                                      (* Uni *) (fun i => result.Stuck)
-                                      (* Cust *) (fun _ => result.Stuck)
-                                      e1
-                   | result.Stuck => result.Stuck
-                   end)
-      (* Pi *) (fun _ _ _ => result.Value)
-      (* tt *) result.Value
-      (* unit *) result.Value
-      (* Eq *) (fun _ _ _ _ _ _ => result.Value)
-      (* Uni *) (fun i => result.Value)
-      (* Cust *) (fun _ => result.Value)
-      e
-  .
-
-  Lemma f_t :
-    forall e, match f e with
-         | result.Step e' => t e e'
-         | result.Value => value.t e
-         | result.Stuck => (forall e', ~ t e e') /\ ~ value.t e
-         end.
-  Proof.
-    induction e using expr.rec0; simpl; auto.
-    - destruct (f e1).
-      + auto.
-      + invcs IHe1; intuition; invc H; inv_existT; try solve_by_inversion.
-      + intuition; invc H1; inv_existT; eauto.
-  Qed.
-End step.
-
-Module star.
-  Definition t : expr.t 0 -> expr.t 0 -> Prop := Relation_Operators.clos_refl_trans_1n _ step.t.
-End star.
-
-Module eval.
-  Definition t (e : expr.t 0) (v : expr.t 0) : Prop :=
-    star.t e v /\ value.t v.
-End eval.
